CODIGO/SUMA/Transformations/ParticionNatToParticionInt.dfy
@@ -1,0 +1,79 @@
+include "../Auxiliar/Sum.dfy"
+include "../Problems/ParticionNat.dfy"
+include "../Problems/ParticionInt.dfy"
+
+function multisetNatToInt(A : multiset<nat>) : (r:(multiset<int>))
+    requires forall e | e in A :: e >= 0
+    ensures A == r;
+
+{
+    if A == multiset{} then multiset{}
+    else var i := minInt(A) as int; multiset{i} + multisetNatToInt(A-multiset{i})
+}
+
+lemma SumNatEqualsSumInt (A:multiset<nat>, B: multiset<int>)
+    requires forall e | e in B :: e >= 0
+    requires A == B
+    ensures GSumNat(A) == GSumInt(B)
+{   
+    if (A == multiset{}) {
+        assert B == multiset{};
+        assert GSumNat(A) == GSumInt(B);
+    }
+    else {
+        var ai := minNat(A);
+        var bi := minInt(B);
+        SumNatEqualsSumInt(A-multiset{ai}, B-multiset{bi});
+        assert ai == bi && GSumNat(A-multiset{ai}) == GSumInt(B-multiset{bi}); 
+        GSumNatPartes(A,multiset{ai},A-multiset{ai}); GSumIntPartes(B,multiset{bi},B-multiset{bi});
+        assert GSumNat(A) == GSumInt(B);
+         
+    }
+}
+
+    
+
+function ParticionNat_to_ParticionInt(A:multiset<nat>) : (r:(multiset<int>))
+{
+    (A)
+}
+
+lemma ParticionNat_ParticionInt(A:multiset<nat>)
+  ensures var PA:= ParticionNat_to_ParticionInt(A);
+          ParticionNat(A) <==> ParticionInt(PA)
+{ 
+    ParticionNat_ParticionInt1(A);
+    ParticionNat_ParticionInt2(A);
+}
+
+lemma ParticionNat_ParticionInt1(A:multiset<nat>)
+    ensures var PA := ParticionNat_to_ParticionInt(A);
+          ParticionNat(A) <== ParticionInt(PA)
+{   
+    var PA := ParticionNat_to_ParticionInt(A);
+    if (ParticionInt(PA)) {
+        var IP1:multiset<int>,IP2:multiset<int> :| IP1 <= PA && IP2 <= PA && IP1 + IP2 == PA && GSumInt(IP1) == GSumInt(IP2);
+
+        var NP1:multiset<nat> := IP1; var NP2:multiset<nat> := IP2; 
+
+        var test1:multiset<nat> := multiset{1,2}; var test2:multiset<int> := multiset{1,2};
+
+        assume GSumNat(NP1) == GSumNat(NP2);
+        assert NP1 <= A && NP2 <= A && NP1 + NP2 == A && GSumNat(NP1) == GSumNat(NP2);
+    }
+}
+
+lemma ParticionNat_ParticionInt2(A:multiset<nat>)
+    ensures var PA := ParticionNat_to_ParticionInt(A);
+          ParticionNat(A) ==> ParticionInt(PA)
+{
+    if (ParticionNat(A)) {
+        var PA := ParticionNat_to_ParticionInt(A);
+        var NP1:multiset<nat>,NP2:multiset<nat> :| NP1 <= A && NP2 <= A && NP1 + NP2 == A && GSumNat(NP1) == GSumNat(NP2);
+
+        var IP1:multiset<int> := NP1; var IP2:multiset<int> := NP2; 
+
+        SumNatEqualsSumInt(NP1,IP1); SumNatEqualsSumInt(NP2,IP2);
+        assert IP1 <= PA && IP2 <= PA && IP1 + IP2 == PA && GSumInt(IP1) == GSumInt(IP2);
+    }
+}
